inductive_proof/Framework.fst
@@ -37,20 +37,6 @@ let rec is_interleaving (l l1 l2:log)
           is_interleaving l' prefix1 l2 /\
           l == Seq.snoc l' last1)))
 
-let add_lastop (lca s1:st) (last1:op_t)
-  : Lemma (requires is_prefix (ops_of lca) (ops_of s1) /\
-                    is_prefix (ops_of lca) (snoc (ops_of s1) last1) /\
-                    (exists l. v_of s1 == apply_log (v_of lca) l)) 
-          (ensures (exists l. do (v_of s1) last1 == apply_log (v_of lca) l)) = 
-  split_prefix init_st (ops_of lca) (ops_of s1); 
-  split_prefix init_st (ops_of lca) (snoc (ops_of s1) last1);
-  lem_apply_log init_st (snoc (ops_of s1) last1);
-  un_snoc_snoc (ops_of s1) last1;
-  assert (fst (un_snoc (snoc (ops_of s1) last1)) = (ops_of s1));
-  assert (apply_log init_st (snoc (ops_of s1) last1) == do (apply_log init_st (ops_of s1)) last1); 
-  assert (do (v_of s1) last1 == apply_log init_st (snoc (ops_of s1) last1));
-  assert (do (v_of s1) last1 == apply_log (v_of lca) (diff (snoc (ops_of s1) last1) (ops_of lca))); ()
-
 let interleaving_predicate (l:log) (lca s1:st)
   (s2:st{is_prefix (ops_of lca) (ops_of s1) /\
          is_prefix (ops_of lca) (ops_of s2)}) =
@@ -60,12 +46,11 @@ let interleaving_predicate (l:log) (lca s1:st)
   eq (apply_log (v_of lca) l)
      (concrete_merge (v_of lca) (v_of s1) (v_of s2))
 
+#push-options "--z3rlimit 100"
 let rec linearizable_s1_0''_base (lca s1 s2':st) (last2:op_t)
-  : Lemma (requires consistent_branches lca s1 s2' /\
-                    is_prefix (ops_of lca) (snoc (ops_of s2') last2) /\
+  : Lemma (requires consistent_branches lca s1 (do_st s2' last2) /\
                     ops_of s1 == ops_of lca /\ ops_of s2' == ops_of lca /\
-                    fst last2 > 0 /\
-                    (forall id. mem_id id (ops_of lca) ==> lt id (fst last2)))
+                    fst last2 > 0)
           (ensures eq (do (v_of s2') last2) (concrete_merge (v_of lca) (v_of s1) (do (v_of s2') last2)))
           (decreases %[length (ops_of lca)]) =
   if length (ops_of lca) = 0 then
@@ -74,36 +59,36 @@ let rec linearizable_s1_0''_base (lca s1 s2':st) (last2:op_t)
     (let l' = inverse_st lca in
      let s1' = inverse_st s1 in
      let s2'' = inverse_st s2' in
+     distinct_snoc_inv (ops_of s2') last2;
      linearizable_s1_0''_base l' s1' s2'' last2;
      linearizable_s1_0''_base_ind lca s1 s2' last2)
 
 let rec linearizable_s1_0'' (lca s1 s2':st) (last2:op_t)
-  : Lemma (requires consistent_branches lca s1 s2' /\
-                    is_prefix (ops_of lca) (snoc (ops_of s2') last2) /\
+  : Lemma (requires consistent_branches lca s1 (do_st s2' last2) /\
+                    is_prefix (ops_of lca) (ops_of s2') /\
                     ops_of s1 = ops_of lca /\                    
-                    fst last2 > 0 /\
-                    (forall id. mem_id id (ops_of lca) ==> lt id (fst last2)))
-          (ensures (exists l2. (do (v_of s2') last2 == apply_log (v_of lca) l2)) /\
-                   eq (do (v_of s2') last2) (concrete_merge (v_of lca) (v_of s1) (do (v_of s2') last2)))
+                    fst last2 > 0)
+          (ensures eq (do (v_of s2') last2) (concrete_merge (v_of lca) (v_of s1) (do (v_of s2') last2)))
           (decreases %[length (ops_of s2')]) = 
   if ops_of s2' = ops_of lca then
     linearizable_s1_0''_base lca s1 s2' last2
   else 
-    (let inv2 = inverse_st s2' in
+    (assert (length (ops_of s2') > length (ops_of lca));
+    let s2'' = inverse_st s2' in
+    distinct_snoc_inv (ops_of s2') last2;
     lem_inverse (ops_of lca) (ops_of s2');
-    lastop_diff (ops_of lca) (ops_of s2');
-    inverse_diff_id_s2' (ops_of lca) (ops_of s1) (ops_of s2');
-    split_prefix init_st (ops_of lca) (ops_of s2');
-    add_lastop lca s2' last2; // ((exists l2. (do (v_of inv2) last2 == apply_log (v_of lca) l2))); 
-    linearizable_s1_0'' lca s1 inv2 last2;
+    split_prefix init_st (ops_of lca) (snoc (ops_of s2'') last2);
+    lt_snoc (ops_of lca) (ops_of s2') last2;
+    s1s2'_snoc (ops_of lca) (ops_of s1) (ops_of s2') last2;
+    assert (consistent_branches lca s1 (do_st s2'' last2));
+    linearizable_s1_0'' lca s1 s2'' last2;
     linearizable_s1_0''_ind lca s1 s2' last2)
 
 let linearizable_s1_0' (lca s1 s2:st)
-  : Lemma (requires consistent_branches_s2_gt0 lca s1 s2 /\
+  : Lemma (requires consistent_branches lca s1 s2 /\
+                    length (ops_of s2) > length (ops_of lca) /\
                     ops_of s1 = ops_of lca)
-          (ensures (exists l1. v_of s1 == apply_log (v_of lca) l1) /\
-                   (exists l2. v_of s2 == apply_log (v_of lca) l2) /\
-                   eq (v_of s2) (concrete_merge (v_of lca) (v_of s1) (v_of s2))) =
+          (ensures eq (v_of s2) (concrete_merge (v_of lca) (v_of s1) (v_of s2))) =
   let pre2, last2 = un_snoc (ops_of s2) in
   split_prefix init_st (ops_of lca) (snoc pre2 last2); 
   lem_inverse (ops_of lca) (ops_of s2);
@@ -125,23 +110,21 @@ let linearizable_s1_0 (lca s1 s2:st)
   split_prefix init_st (ops_of lca) (ops_of s2);
   if ops_of s2 = ops_of lca then
     linearizable_s1_0_s2_0_base lca s1 s2 
-  else linearizable_s1_0' lca s1 s2
+  else (linearizable_s1_0' lca s1 s2)
 
 let linearizable_s2_0' (lca s1 s2:st)
   : Lemma (requires consistent_branches_s1_gt0 lca s1 s2 /\
                     ops_of s2 = ops_of lca)
-          (ensures (exists l1. v_of s1 == apply_log (v_of lca) l1) /\
-                   (exists l2. v_of s2 == apply_log (v_of lca) l2) /\
-                   eq (v_of s1) (concrete_merge (v_of lca) (v_of s1) (v_of s2))) =
+          (ensures eq (v_of s1) (concrete_merge (v_of lca) (v_of s1) (v_of s2))) =
   linearizable_s1_0' lca s2 s1;
-    //assert ((exists l1. v_of s1 == apply_log (v_of lca) l1) /\ (exists l2. v_of s2 == apply_log (v_of lca) l2));
+               //assert ((exists l1. v_of s1 == apply_log (v_of lca) l1) /\ (exists l2. v_of s2 == apply_log (v_of lca) l2));
   merge_is_comm lca s1 s2;
-    //assert (eq (concrete_merge (v_of lca) (v_of s1) (v_of s2)) 
+               //assert (eq (concrete_merge (v_of lca) (v_of s1) (v_of s2)) 
                //(concrete_merge (v_of lca) (v_of s2) (v_of s1))); 
-    //assert (eq (v_of s1) (concrete_merge (v_of lca) (v_of s2) (v_of s1)));
+               //assert (eq (v_of s1) (concrete_merge (v_of lca) (v_of s2) (v_of s1)));
   symmetric (concrete_merge (v_of lca) (v_of s1) (v_of s2)) (concrete_merge (v_of lca) (v_of s2) (v_of s1));
   transitive (v_of s1) (concrete_merge (v_of lca) (v_of s2) (v_of s1)) (concrete_merge (v_of lca) (v_of s1) (v_of s2));
-    //assert (eq (v_of s1) (concrete_merge (v_of lca) (v_of s1) (v_of s2)));  
+               //assert (eq (v_of s1) (concrete_merge (v_of lca) (v_of s1) (v_of s2)));  
   ()
 
 let linearizable_s2_0 (lca s1 s2:st)
@@ -154,191 +137,164 @@ let linearizable_s2_0 (lca s1 s2:st)
   else linearizable_s2_0' lca s1 s2
 
 let rec linearizable_gt0_s2'_s10 (lca s1 s2:st) (last1 last2:op_t)
-  : Lemma (requires consistent_branches lca s1 s2 /\
+  : Lemma (requires consistent_branches lca (do_st s1 last1) (do_st s2 last2) /\
+                    consistent_branches lca (do_st s1 last1) s2 /\
+                    consistent_branches lca s1 s2 /\
                     ops_of s1 = ops_of lca /\
                     fst last1 <> fst last2 /\
-                    distinct_ops (snoc (ops_of s1) last1) /\
-                    distinct_ops (snoc (ops_of s2) last2) /\
                     Second_then_first? (resolve_conflict last1 last2))                   
-          (ensures (exists l2. (do (v_of s2) last2 == apply_log (v_of lca) l2)) /\
-                   (exists l2. (v_of s2) == apply_log (v_of lca) l2) /\
-                   (exists l1. (do (v_of s1) last1 == apply_log (v_of lca) l1)) /\
-                    eq (do (concrete_merge (v_of lca) (do (v_of s1) last1) (v_of s2)) last2)
-                       (concrete_merge (v_of lca) (do (v_of s1) last1) (do (v_of s2) last2)))
+          (ensures eq (do (concrete_merge (v_of lca) (do (v_of s1) last1) (v_of s2)) last2)
+                      (concrete_merge (v_of lca) (do (v_of s1) last1) (do (v_of s2) last2)))
           (decreases  %[length (ops_of s2)]) = 
-  split_prefix init_st (ops_of lca) (ops_of s2); // (exists l2. (v_of s2) == apply_log (v_of lca) l2);
-  add_lastop lca s2 last2; //(exists l2. (do (v_of s2) last2 == apply_log (v_of lca) l2)); 
-  add_lastop lca s1 last1; //(exists l1. (do (v_of s1) last1 == apply_log (v_of lca) l1)));
-  
   if ops_of s2 = ops_of lca then
      linearizable_gt0_base lca s1 s2 last1 last2
   else 
-    (let s2' = inverse_st s2 in
+    (assert (length (ops_of s2) > length (ops_of lca)); 
+     let s2' = inverse_st s2 in
      lem_inverse (ops_of lca) (ops_of s2);
      lastop_diff (ops_of lca) (ops_of s2);
-     inverse_diff_id_s2' (ops_of lca) (ops_of s1) (ops_of s2);
-     lemma_append_count_assoc_fst (ops_of s2) (create 1 last2);
-     let pre, lastop = un_snoc (ops_of s2) in
-     lemma_append_count_assoc_fst pre (create 1 lastop);
-     distinct_append pre (create 1 last2);
+     inverse_diff_id_s2' (ops_of lca) (snoc (ops_of s1) last1) (ops_of s2);
+     split_prefix init_st (ops_of lca) (ops_of s2');
+     assert (consistent_branches lca (do_st s1 last1) s2');
+
+     distinct_snoc_inv (ops_of s2) last2;
+     split_prefix init_st (ops_of lca) (snoc (ops_of s2') last2);
+     lt_snoc (ops_of lca) (ops_of s2) last2; 
+     s1s2'_snoc (ops_of lca) (snoc (ops_of s1) last1) (ops_of s2) last2;
+     assert (consistent_branches lca (do_st s1 last1) (do_st s2' last2));
+
      linearizable_gt0_s2'_s10 lca s1 s2' last1 last2;
      linearizable_gt0_ind lca s1 s2 last1 last2)
 
 let rec linearizable_gt0_s2' (lca s1 s2:st) (last1 last2:op_t)
-  : Lemma (requires consistent_branches lca s1 s2 /\
+  : Lemma (requires consistent_branches lca (do_st s1 last1) (do_st s2 last2) /\
+                    consistent_branches lca (do_st s1 last1) s2 /\
+                    consistent_branches lca s1 s2 /\
+                    is_prefix (ops_of lca) (ops_of s1) /\
                     fst last1 <> fst last2 /\
-                    distinct_ops (snoc (ops_of s1) last1) /\
-                    distinct_ops (snoc (ops_of s2) last2) /\
                     Second_then_first? (resolve_conflict last1 last2))
-          (ensures (exists l2. (do (v_of s2) last2 == apply_log (v_of lca) l2)) /\
-                   (exists l2. (v_of s2) == apply_log (v_of lca) l2) /\
-                   (exists l1. (v_of s1) == apply_log (v_of lca) l1) /\
-                   (exists l1. (do (v_of s1) last1 == apply_log (v_of lca) l1)) /\
-                   eq (do (concrete_merge (v_of lca) (do (v_of s1) last1) (v_of s2)) last2)
+          (ensures eq (do (concrete_merge (v_of lca) (do (v_of s1) last1) (v_of s2)) last2)
                        (concrete_merge (v_of lca) (do (v_of s1) last1) (do (v_of s2) last2)))
           (decreases %[length (ops_of s1); length (ops_of s2)]) = 
-  split_prefix init_st (ops_of lca) (ops_of s2); // (exists l2. (v_of s2) == apply_log (v_of lca) l2);
-  split_prefix init_st (ops_of lca) (ops_of s1); // (exists l1. (v_of s1) == apply_log (v_of lca) l1);
-  add_lastop lca s2 last2; //(exists l2. (do (v_of s2) last2 == apply_log (v_of lca) l2)); 
-  add_lastop lca s1 last1; //(exists l1. (do (v_of s1) last1 == apply_log (v_of lca) l1)));
-  
   if ops_of s1 = ops_of lca && ops_of s2 = ops_of lca then
     linearizable_gt0_base lca s1 s2 last1 last2 
   else if ops_of s1 = ops_of lca then
     linearizable_gt0_s2'_s10 lca s1 s2 last1 last2 
-  else (let s1' = inverse_st s1 in
+  else (assert (length (ops_of s1) > length (ops_of lca));
+        let s1' = inverse_st s1 in
+        distinct_snoc_inv (ops_of s1) last1;
         lem_inverse (ops_of lca) (ops_of s1);
+        split_prefix init_st (ops_of lca) (snoc (ops_of s1') last1);
+        lt_snoc (ops_of lca) (ops_of s1) last1; 
+        s1's2_snoc (ops_of lca) (ops_of s1) (ops_of s2) last1;   
+        s1's2_snoc (ops_of lca) (ops_of s1) (snoc (ops_of s2) last2) last1;   
         lastop_diff (ops_of lca) (ops_of s1);
         inverse_diff_id_s1' (ops_of lca) (ops_of s1) (ops_of s2);
-        lemma_append_count_assoc_fst (ops_of s1) (create 1 last1);
-        let pre, lastop = un_snoc (ops_of s1) in
-        lemma_append_count_assoc_fst pre (create 1 lastop);
-        distinct_append pre (create 1 last1);
+        split_prefix init_st (ops_of lca) (ops_of s1');
+               
         linearizable_gt0_s2' lca s1' s2 last1 last2;
         linearizable_gt0_ind1 lca s1 s2 last1 last2)  
 
 let linearizable_gt0_s2 (lca s1 s2:st)
   : Lemma (requires consistent_branches_s1s2_gt0 lca s1 s2 /\
+                    consistent_branches lca s1 (inverse_st s2) /\
+                    consistent_branches lca (inverse_st s1) (inverse_st s2) /\
                     (let _, last1 = un_snoc (ops_of s1) in
                     let _, last2 = un_snoc (ops_of s2) in
                     fst last1 <> fst last2 /\
-                    Second_then_first? (resolve_conflict last1 last2) /\
-                    (exists l2. (v_of (inverse_st s2) == apply_log (v_of lca) l2)) /\
-                    (exists l2. (v_of s2) == apply_log (v_of lca) l2) /\
-                    (exists l1. (v_of s1) == apply_log (v_of lca) l1)))
+                    Second_then_first? (resolve_conflict last1 last2)))
           (ensures (let pre2, last2 = un_snoc (ops_of s2) in                   
                    eq (do (concrete_merge (v_of lca) (v_of s1) (v_of (inverse_st s2))) last2)
-                       (concrete_merge (v_of lca) (v_of s1) (v_of s2)))) = 
-  let pre2, last2 = un_snoc (ops_of s2) in
+                      (concrete_merge (v_of lca) (v_of s1) (v_of s2)))) = 
+  let _, last2 = un_snoc (ops_of s2) in
   let _, last1 = un_snoc (ops_of s1) in
-  assert (v_of s2 == do (v_of (inverse_st s2)) last2);
-  assert (v_of s1 == do (v_of (inverse_st s1)) last1);
-  lem_inverse (ops_of lca) (ops_of s2);
-  lem_inverse (ops_of lca) (ops_of s1);
-  lastop_diff (ops_of lca) (ops_of s2);
-  lastop_diff (ops_of lca) (ops_of s1);
-  inverse_diff_id_s1'_s2' (ops_of lca) (ops_of s1) (ops_of s2);
   linearizable_gt0_s2' lca (inverse_st s1) (inverse_st s2) last1 last2
 
 let rec linearizable_gt0_s1'_s20 (lca s1 s2:st) (last1 last2:op_t)
-  : Lemma (requires consistent_branches lca s1 s2 /\
+  : Lemma (requires consistent_branches lca (do_st s1 last1) (do_st s2 last2) /\
+                    consistent_branches lca s1 (do_st s2 last2) /\
+                    consistent_branches lca s1 s2 /\
                     ops_of s2 = ops_of lca /\
                     fst last1 <> fst last2 /\
-                    distinct_ops (snoc (ops_of s1) last1) /\
-                    distinct_ops (snoc (ops_of s2) last2) /\
                     First_then_second? (resolve_conflict last1 last2))
-          (ensures (exists l2. (do (v_of s2) last2 == apply_log (v_of lca) l2)) /\
-                   (exists l1. (v_of s1) == apply_log (v_of lca) l1) /\
-                   (exists l1. (do (v_of s1) last1 == apply_log (v_of lca) l1)) /\
-                   eq (do (concrete_merge (v_of lca) (v_of s1) (do (v_of s2) last2)) last1)
+          (ensures eq (do (concrete_merge (v_of lca) (v_of s1) (do (v_of s2) last2)) last1)
                        (concrete_merge (v_of lca) (do (v_of s1) last1) (do (v_of s2) last2)))
           (decreases  %[length (ops_of s1)]) =
-  split_prefix init_st (ops_of lca) (ops_of s1); // (exists l1. (v_of s1) == apply_log (v_of lca) l1);
-  add_lastop lca s2 last2; //(exists l2. (do (v_of s2) last2 == apply_log (v_of lca) l2)); 
-  add_lastop lca s1 last1; //(exists l1. (do (v_of s1) last1 == apply_log (v_of lca) l1)));
-  
   if ops_of s1 = ops_of lca then
      linearizable_gt0_base lca s1 s2 last1 last2
   else 
-    (let s1' = inverse_st s1 in
+    (assert (length (ops_of s1) > length (ops_of lca));
+     let s1' = inverse_st s1 in
      lem_inverse (ops_of lca) (ops_of s1);
      lastop_diff (ops_of lca) (ops_of s1);
-     inverse_diff_id_s1' (ops_of lca) (ops_of s1) (ops_of s2);
-     lemma_append_count_assoc_fst (ops_of s1) (create 1 last1);
-     let pre, lastop = un_snoc (ops_of s1) in
-     lemma_append_count_assoc_fst pre (create 1 lastop);
-     distinct_append pre (create 1 last1);
+     inverse_diff_id_s1' (ops_of lca) (ops_of s1) (snoc (ops_of s2) last2);
+     split_prefix init_st (ops_of lca) (ops_of s1');
+     assert (consistent_branches lca s1' (do_st s2 last2)); 
+
+     distinct_snoc_inv (ops_of s1) last1;
+     split_prefix init_st (ops_of lca) (snoc (ops_of s1') last1);
+     lt_snoc (ops_of lca) (ops_of s1) last1; 
+     s1's2_snoc (ops_of lca) (ops_of s1) (snoc (ops_of s2) last2) last1;
+     assert (consistent_branches lca (do_st s1' last1) (do_st s2 last2));
+     
      linearizable_gt0_s1'_s20 lca s1' s2 last1 last2;
      linearizable_gt0_ind1 lca s1 s2 last1 last2)
 
 let rec linearizable_gt0_s1' (lca s1 s2:st) (last1 last2:op_t)
-  : Lemma (requires consistent_branches lca s1 s2 /\
+  : Lemma (requires consistent_branches lca (do_st s1 last1) (do_st s2 last2) /\
+                    consistent_branches lca s1 (do_st s2 last2) /\
+                    consistent_branches lca s1 s2 /\
+                    is_prefix (ops_of lca) (ops_of s2) /\
                     fst last1 <> fst last2 /\
-                    distinct_ops (snoc (ops_of s1) last1) /\
-                    distinct_ops (snoc (ops_of s2) last2) /\
                     First_then_second? (resolve_conflict last1 last2))
-          (ensures (exists l2. (do (v_of s2) last2 == apply_log (v_of lca) l2)) /\
-                   (exists l2. (v_of s2) == apply_log (v_of lca) l2) /\
-                   (exists l1. (v_of s1) == apply_log (v_of lca) l1) /\
-                   (exists l1. (do (v_of s1) last1 == apply_log (v_of lca) l1)) /\
-                   eq (do (concrete_merge (v_of lca) (v_of s1) (do (v_of s2) last2)) last1)
-                       (concrete_merge (v_of lca) (do (v_of s1) last1) (do (v_of s2) last2)))
+          (ensures eq (do (concrete_merge (v_of lca) (v_of s1) (do (v_of s2) last2)) last1)
+                      (concrete_merge (v_of lca) (do (v_of s1) last1) (do (v_of s2) last2)))
           (decreases %[length (ops_of s2); length (ops_of s1)]) =
-  split_prefix init_st (ops_of lca) (ops_of s2); // (exists l2. (v_of s2) == apply_log (v_of lca) l2);
-  split_prefix init_st (ops_of lca) (ops_of s1); // (exists l1. (v_of s1) == apply_log (v_of lca) l1);
-  add_lastop lca s2 last2; //(exists l2. (do (v_of s2) last2 == apply_log (v_of lca) l2)); 
-  add_lastop lca s1 last1; //(exists l1. (do (v_of s1) last1 == apply_log (v_of lca) l1)));
-  
   if ops_of s1 = ops_of lca && ops_of s2 = ops_of lca then
     linearizable_gt0_base lca s1 s2 last1 last2 
   else if ops_of s2 = ops_of lca then
     linearizable_gt0_s1'_s20 lca s1 s2 last1 last2 
-  else (let s2' = inverse_st s2 in
+  else (assert (length (ops_of s2) > length (ops_of lca));
+        let s2' = inverse_st s2 in
+        distinct_snoc_inv (ops_of s2) last2;
         lem_inverse (ops_of lca) (ops_of s2);
+        split_prefix init_st (ops_of lca) (snoc (ops_of s2') last2);
+        lt_snoc (ops_of lca) (ops_of s2) last2; 
+        s1s2'_snoc (ops_of lca) (ops_of s1) (ops_of s2) last2;   
+        s1s2'_snoc (ops_of lca) (snoc (ops_of s1) last1) (ops_of s2) last2; 
         lastop_diff (ops_of lca) (ops_of s2);
         inverse_diff_id_s2' (ops_of lca) (ops_of s1) (ops_of s2);
-        lemma_append_count_assoc_fst (ops_of s2) (create 1 last2);
-        let pre, lastop = un_snoc (ops_of s2) in
-        lemma_append_count_assoc_fst pre (create 1 lastop);
-        distinct_append pre (create 1 last2);
+        split_prefix init_st (ops_of lca) (ops_of s2');
+        
         linearizable_gt0_s1' lca s1 s2' last1 last2;
         linearizable_gt0_ind lca s1 s2 last1 last2) 
 
 let linearizable_gt0_s1 (lca s1 s2:st)
   : Lemma (requires consistent_branches_s1s2_gt0 lca s1 s2 /\
+                    consistent_branches lca (inverse_st s1) s2 /\
+                    consistent_branches lca (inverse_st s1) (inverse_st s2) /\
                     (let _, last1 = un_snoc (ops_of s1) in
                     let _, last2 = un_snoc (ops_of s2) in
                     fst last1 <> fst last2 /\
-                    First_then_second? (resolve_conflict last1 last2) /\
-                    (exists l1. (v_of (inverse_st s1) == apply_log (v_of lca) l1)) /\
-                    (exists l2. (v_of s2) == apply_log (v_of lca) l2) /\
-                    (exists l1. (v_of s1) == apply_log (v_of lca) l1)))
+                    First_then_second? (resolve_conflict last1 last2)))
           (ensures (let _, last1 = un_snoc (ops_of s1) in
                    eq (do (concrete_merge (v_of lca) (v_of (inverse_st s1)) (v_of s2)) last1)
                        (concrete_merge (v_of lca) (v_of s1) (v_of s2)))) = 
   let _, last2 = un_snoc (ops_of s2) in
-  let pre1, last1 = un_snoc (ops_of s1) in
-  assert (v_of s2 == do (v_of (inverse_st s2)) last2);
-  assert (v_of s1 == do (v_of (inverse_st s1)) last1);
-  lem_inverse (ops_of lca) (ops_of s2);
-  lem_inverse (ops_of lca) (ops_of s1);
-  lastop_diff (ops_of lca) (ops_of s2);
-  lastop_diff (ops_of lca) (ops_of s1);
-  inverse_diff_id_s1'_s2' (ops_of lca) (ops_of s1) (ops_of s2);
+  let _, last1 = un_snoc (ops_of s1) in
   linearizable_gt0_s1' lca (inverse_st s1) (inverse_st s2) last1 last2
 
 let linearizable_gt0 (lca s1 s2:st)
   : Lemma (requires consistent_branches_s1s2_gt0 lca s1 s2 /\
+                    consistent_branches lca (inverse_st s1) (inverse_st s2) /\
                     (let _, last1 = un_snoc (ops_of s1) in
                     let _, last2 = un_snoc (ops_of s2) in
                     fst last1 <> fst last2 /\
-                    (exists l2. (v_of s2) == apply_log (v_of lca) l2) /\
-                    (exists l1. (v_of s1) == apply_log (v_of lca) l1) /\
                     (First_then_second? (resolve_conflict last1 last2) ==>
-                       (exists l1. (v_of (inverse_st s1) == apply_log (v_of lca) l1))) /\
+                       consistent_branches lca (inverse_st s1) s2) /\
 
                     (Second_then_first? (resolve_conflict last1 last2) ==>
-                       (exists l2. (v_of (inverse_st s2) == apply_log (v_of lca) l2)))))
+                       consistent_branches lca s1 (inverse_st s2))))
           (ensures (let _, last1 = un_snoc (ops_of s1) in
                     let _, last2 = un_snoc (ops_of s2) in
                     (First_then_second? (resolve_conflict last1 last2) ==>
@@ -381,22 +337,25 @@ let interleaving_helper_inv2 (lca s1 s2 l':log)
 
 let interleaving_s1_inv (lca s1 s2:st) (l':log)
   : Lemma (requires consistent_branches_s1s2_gt0 lca s1 s2 /\
-                    is_prefix (ops_of lca) (ops_of (inverse_st s1)) /\
                     interleaving_predicate l' lca (inverse_st s1) s2 /\
                     (let _, last1 = un_snoc (ops_of s1) in
                      let _, last2 = un_snoc (ops_of s2) in
                      fst last1 <> fst last2 /\
                      First_then_second? (resolve_conflict last1 last2)) /\
-                     (exists l2. (v_of s2) == apply_log (v_of lca) l2) /\
-                     (exists l1. (v_of s1) == apply_log (v_of lca) l1) /\
-                     (exists l1. (v_of (inverse_st s1) == apply_log (v_of lca) l1)))
+                     consistent_branches lca (inverse_st s1) s2)
           (ensures (let _, last1 = un_snoc (ops_of s1) in
                     let l = Seq.snoc l' last1 in
                     interleaving_predicate l lca s1 s2 /\
                     (exists l. interleaving_predicate l lca s1 s2))) = 
   let pre1, last1 = un_snoc (ops_of s1) in
+  let pre2, last2 = un_snoc (ops_of s2) in
   let l = Seq.snoc l' last1 in
   interleaving_helper_inv1 (ops_of lca) (ops_of s1) (ops_of s2) l'; 
+  lem_inverse (ops_of lca) (ops_of s1); lem_inverse (ops_of lca) (ops_of s2);
+  lastop_diff (ops_of lca) (ops_of s1); lastop_diff (ops_of lca) (ops_of s2);
+  inverse_diff_id_s1'_s2' (ops_of lca) (ops_of s1) (ops_of s2);
+  split_prefix init_st (ops_of lca) pre1;
+  split_prefix init_st (ops_of lca) pre2;
   linearizable_gt0 lca s1 s2; 
   symmetric (apply_log (v_of lca) l')
             (concrete_merge (v_of lca) (v_of (inverse_st s1)) (v_of s2));
@@ -409,22 +368,25 @@ let interleaving_s1_inv (lca s1 s2:st) (l':log)
 
 let interleaving_s2_inv (lca s1 s2:st) (l':log)
   : Lemma (requires consistent_branches_s1s2_gt0 lca s1 s2 /\
-                    is_prefix (ops_of lca) (ops_of (inverse_st s2)) /\
                     interleaving_predicate l' lca s1 (inverse_st s2) /\
                     (let _, last1 = un_snoc (ops_of s1) in
                      let _, last2 = un_snoc (ops_of s2) in
                      fst last1 <> fst last2 /\
                      Second_then_first? (resolve_conflict last1 last2)) /\
-                     (exists l2. (v_of s2) == apply_log (v_of lca) l2) /\
-                     (exists l1. (v_of s1) == apply_log (v_of lca) l1) /\
-                     (exists l2. (v_of (inverse_st s2) == apply_log (v_of lca) l2)))
+                     consistent_branches lca s1 (inverse_st s2))
           (ensures (let _, last2 = un_snoc (ops_of s2) in
                     let l = Seq.snoc l' last2 in
                     interleaving_predicate l lca s1 s2 /\
                     (exists l. interleaving_predicate l lca s1 s2))) = 
+  let pre1, last1 = un_snoc (ops_of s1) in
   let pre2, last2 = un_snoc (ops_of s2) in
   let l = Seq.snoc l' last2 in
   interleaving_helper_inv2 (ops_of lca) (ops_of s1) (ops_of s2) l'; 
+  lem_inverse (ops_of lca) (ops_of s1); lem_inverse (ops_of lca) (ops_of s2);
+  lastop_diff (ops_of lca) (ops_of s1); lastop_diff (ops_of lca) (ops_of s2);
+  inverse_diff_id_s1'_s2' (ops_of lca) (ops_of s1) (ops_of s2);
+  split_prefix init_st (ops_of lca) pre1;
+  split_prefix init_st (ops_of lca) pre2;
   linearizable_gt0 lca s1 s2;
   symmetric (apply_log (v_of lca) l')
             (concrete_merge (v_of lca) (v_of s1) (v_of (inverse_st s2)));
@@ -514,7 +476,7 @@ let rec linearizable (lca s1 s2:st)
         end
         
         else 
-        begin
+        begin 
           linearizable_s2_gt0_pre lca s1 s2;
           split_prefix init_st (ops_of lca) pre2;
           linearizable lca s1 inv2;
@@ -530,3 +492,4 @@ let rec linearizable (lca s1 s2:st)
           end
         end
       end
+#pop-options
